Bring lemmas into compliance with the schemes

su.nsk.iae.rpl/src/su/nsk/iae/rpl/generator/Main.java
@@ -152,7 +152,6 @@ public class Main {
 							partEinvPatternDef.getSimpleFmParams(),
 							partEinvPatternDef.getRegFmParams(),
 							new ArrayList<>(),
-							null,
 							s,
 							sPrimed
 							);
@@ -180,7 +179,6 @@ public class Main {
 							partEinvPatternDef.getSimpleFmParams(),
 							partEinvPatternDef.getRegFmParams(),
 							partReqPatternDef.getRegFmParams(),
-							null,
 							s,
 							sPrimed
 							);
